language/move-prover/bytecode-to-boogie/tests/translator_tests.rs
@@ -42,6 +42,11 @@ fn test_struct() {
 }
 
 #[test]
+fn test_aborts_if() {
+    test(VERIFY, &["test_mvir/test-aborts-if.mvir"]);
+}
+
+#[test]
 fn test_lib() {
     test(
         NO_VERIFY,
