language/move-prover/bytecode-to-boogie/tests/goldenfiles/test-aborts-if.bpl
@@ -1,0 +1,572 @@
+
+
+// ** structs of module TestAbortIf
+
+
+
+// ** functions of module TestAbortIf
+
+procedure {:inline 1} TestAbortIf_abort1 (arg0: Value, arg1: Value) returns ()
+requires ExistsTxnSenderAccount(m, txn);
+ensures old(!(b#Boolean(Boolean(i#Integer(arg0) <= i#Integer(arg1))))) ==> !abort_flag;
+ensures old(b#Boolean(Boolean(i#Integer(arg0) <= i#Integer(arg1)))) ==> abort_flag;
+{
+    // declare local variables
+    var t0: Value; // IntegerType()
+    var t1: Value; // IntegerType()
+    var t2: Value; // IntegerType()
+    var t3: Value; // IntegerType()
+    var t4: Value; // BooleanType()
+    var t5: Value; // BooleanType()
+    var t6: Value; // IntegerType()
+
+    var tmp: Value;
+    var old_size: int;
+
+    var saved_m: Memory;
+    assume !abort_flag;
+    saved_m := m;
+
+    // assume arguments are of correct types
+    assume is#Integer(arg0);
+    assume is#Integer(arg1);
+
+    old_size := local_counter;
+    local_counter := local_counter + 7;
+    m := UpdateLocal(m, old_size + 0, arg0);
+    m := UpdateLocal(m, old_size + 1, arg1);
+
+    // bytecode translation starts here
+    call tmp := CopyOrMoveValue(GetLocal(m, old_size + 0));
+    m := UpdateLocal(m, old_size + 2, tmp);
+
+    call tmp := CopyOrMoveValue(GetLocal(m, old_size + 1));
+    m := UpdateLocal(m, old_size + 3, tmp);
+
+    call tmp := Gt(GetLocal(m, old_size + 2), GetLocal(m, old_size + 3));
+    m := UpdateLocal(m, old_size + 4, tmp);
+
+    call tmp := Not(GetLocal(m, old_size + 4));
+    m := UpdateLocal(m, old_size + 5, tmp);
+
+    tmp := GetLocal(m, old_size + 5);
+    if (!b#Boolean(tmp)) { goto Label_7; }
+
+    call tmp := LdConst(1);
+    m := UpdateLocal(m, old_size + 6, tmp);
+
+    goto Label_Abort;
+
+Label_7:
+    return;
+
+Label_Abort:
+    abort_flag := true;
+    m := saved_m;
+}
+
+procedure TestAbortIf_abort1_verify (arg0: Value, arg1: Value) returns ()
+{
+    call TestAbortIf_abort1(arg0, arg1);
+}
+
+procedure {:inline 1} TestAbortIf_abort2 (arg0: Value, arg1: Value) returns ()
+requires ExistsTxnSenderAccount(m, txn);
+ensures old(!(b#Boolean(Boolean(i#Integer(arg0) <= i#Integer(arg1))))) ==> !abort_flag;
+ensures old(b#Boolean(Boolean(i#Integer(arg0) <= i#Integer(arg1)))) ==> abort_flag;
+{
+    // declare local variables
+    var t0: Value; // IntegerType()
+    var t1: Value; // IntegerType()
+
+    var tmp: Value;
+    var old_size: int;
+
+    var saved_m: Memory;
+    assume !abort_flag;
+    saved_m := m;
+
+    // assume arguments are of correct types
+    assume is#Integer(arg0);
+    assume is#Integer(arg1);
+
+    old_size := local_counter;
+    local_counter := local_counter + 2;
+    m := UpdateLocal(m, old_size + 0, arg0);
+    m := UpdateLocal(m, old_size + 1, arg1);
+
+    // bytecode translation starts here
+    return;
+
+Label_Abort:
+    abort_flag := true;
+    m := saved_m;
+}
+
+procedure TestAbortIf_abort2_verify (arg0: Value, arg1: Value) returns ()
+{
+    call TestAbortIf_abort2(arg0, arg1);
+}
+
+procedure {:inline 1} TestAbortIf_abort3 (arg0: Value, arg1: Value) returns ()
+requires ExistsTxnSenderAccount(m, txn);
+ensures old(!(b#Boolean(Boolean(i#Integer(arg0) <= i#Integer(arg1))))) ==> !abort_flag;
+ensures old(b#Boolean(Boolean(i#Integer(arg0) <= i#Integer(arg1)))) ==> abort_flag;
+{
+    // declare local variables
+    var t0: Value; // IntegerType()
+    var t1: Value; // IntegerType()
+    var t2: Value; // BooleanType()
+    var t3: Value; // BooleanType()
+    var t4: Value; // IntegerType()
+
+    var tmp: Value;
+    var old_size: int;
+
+    var saved_m: Memory;
+    assume !abort_flag;
+    saved_m := m;
+
+    // assume arguments are of correct types
+    assume is#Integer(arg0);
+    assume is#Integer(arg1);
+
+    old_size := local_counter;
+    local_counter := local_counter + 5;
+    m := UpdateLocal(m, old_size + 0, arg0);
+    m := UpdateLocal(m, old_size + 1, arg1);
+
+    // bytecode translation starts here
+    call tmp := LdFalse();
+    m := UpdateLocal(m, old_size + 2, tmp);
+
+    call tmp := Not(GetLocal(m, old_size + 2));
+    m := UpdateLocal(m, old_size + 3, tmp);
+
+    tmp := GetLocal(m, old_size + 3);
+    if (!b#Boolean(tmp)) { goto Label_5; }
+
+    call tmp := LdConst(2);
+    m := UpdateLocal(m, old_size + 4, tmp);
+
+    goto Label_Abort;
+
+Label_5:
+    return;
+
+Label_Abort:
+    abort_flag := true;
+    m := saved_m;
+}
+
+procedure TestAbortIf_abort3_verify (arg0: Value, arg1: Value) returns ()
+{
+    call TestAbortIf_abort3(arg0, arg1);
+}
+
+procedure {:inline 1} TestAbortIf_abort4 (arg0: Value, arg1: Value) returns ()
+requires ExistsTxnSenderAccount(m, txn);
+ensures old(!(b#Boolean(Boolean(i#Integer(arg0) < i#Integer(arg1))))) ==> !abort_flag;
+ensures old(b#Boolean(Boolean(i#Integer(arg0) < i#Integer(arg1)))) ==> abort_flag;
+{
+    // declare local variables
+    var t0: Value; // IntegerType()
+    var t1: Value; // IntegerType()
+    var t2: Value; // IntegerType()
+    var t3: Value; // IntegerType()
+    var t4: Value; // BooleanType()
+    var t5: Value; // BooleanType()
+    var t6: Value; // IntegerType()
+
+    var tmp: Value;
+    var old_size: int;
+
+    var saved_m: Memory;
+    assume !abort_flag;
+    saved_m := m;
+
+    // assume arguments are of correct types
+    assume is#Integer(arg0);
+    assume is#Integer(arg1);
+
+    old_size := local_counter;
+    local_counter := local_counter + 7;
+    m := UpdateLocal(m, old_size + 0, arg0);
+    m := UpdateLocal(m, old_size + 1, arg1);
+
+    // bytecode translation starts here
+    call tmp := CopyOrMoveValue(GetLocal(m, old_size + 0));
+    m := UpdateLocal(m, old_size + 2, tmp);
+
+    call tmp := CopyOrMoveValue(GetLocal(m, old_size + 1));
+    m := UpdateLocal(m, old_size + 3, tmp);
+
+    call tmp := Gt(GetLocal(m, old_size + 2), GetLocal(m, old_size + 3));
+    m := UpdateLocal(m, old_size + 4, tmp);
+
+    call tmp := Not(GetLocal(m, old_size + 4));
+    m := UpdateLocal(m, old_size + 5, tmp);
+
+    tmp := GetLocal(m, old_size + 5);
+    if (!b#Boolean(tmp)) { goto Label_7; }
+
+    call tmp := LdConst(1);
+    m := UpdateLocal(m, old_size + 6, tmp);
+
+    goto Label_Abort;
+
+Label_7:
+    return;
+
+Label_Abort:
+    abort_flag := true;
+    m := saved_m;
+}
+
+procedure TestAbortIf_abort4_verify (arg0: Value, arg1: Value) returns ()
+{
+    call TestAbortIf_abort4(arg0, arg1);
+}
+
+procedure {:inline 1} TestAbortIf_abort5 (arg0: Value, arg1: Value) returns ()
+requires ExistsTxnSenderAccount(m, txn);
+ensures old(!(b#Boolean(Boolean(i#Integer(arg0) <= i#Integer(arg1)))) && (b#Boolean(Boolean(i#Integer(arg0) > i#Integer(arg1))))) ==> !abort_flag;
+ensures old(b#Boolean(Boolean(i#Integer(arg0) <= i#Integer(arg1)))) ==> abort_flag;
+{
+    // declare local variables
+    var t0: Value; // IntegerType()
+    var t1: Value; // IntegerType()
+    var t2: Value; // IntegerType()
+    var t3: Value; // IntegerType()
+    var t4: Value; // BooleanType()
+    var t5: Value; // BooleanType()
+    var t6: Value; // IntegerType()
+
+    var tmp: Value;
+    var old_size: int;
+
+    var saved_m: Memory;
+    assume !abort_flag;
+    saved_m := m;
+
+    // assume arguments are of correct types
+    assume is#Integer(arg0);
+    assume is#Integer(arg1);
+
+    old_size := local_counter;
+    local_counter := local_counter + 7;
+    m := UpdateLocal(m, old_size + 0, arg0);
+    m := UpdateLocal(m, old_size + 1, arg1);
+
+    // bytecode translation starts here
+    call tmp := CopyOrMoveValue(GetLocal(m, old_size + 0));
+    m := UpdateLocal(m, old_size + 2, tmp);
+
+    call tmp := CopyOrMoveValue(GetLocal(m, old_size + 1));
+    m := UpdateLocal(m, old_size + 3, tmp);
+
+    call tmp := Gt(GetLocal(m, old_size + 2), GetLocal(m, old_size + 3));
+    m := UpdateLocal(m, old_size + 4, tmp);
+
+    call tmp := Not(GetLocal(m, old_size + 4));
+    m := UpdateLocal(m, old_size + 5, tmp);
+
+    tmp := GetLocal(m, old_size + 5);
+    if (!b#Boolean(tmp)) { goto Label_7; }
+
+    call tmp := LdConst(1);
+    m := UpdateLocal(m, old_size + 6, tmp);
+
+    goto Label_Abort;
+
+Label_7:
+    return;
+
+Label_Abort:
+    abort_flag := true;
+    m := saved_m;
+}
+
+procedure TestAbortIf_abort5_verify (arg0: Value, arg1: Value) returns ()
+{
+    call TestAbortIf_abort5(arg0, arg1);
+}
+
+procedure {:inline 1} TestAbortIf_abort6 (arg0: Value, arg1: Value) returns ()
+requires ExistsTxnSenderAccount(m, txn);
+ensures old(!(b#Boolean(Boolean(i#Integer(arg0) < i#Integer(arg1)))) && (b#Boolean(Boolean(i#Integer(arg0) > i#Integer(arg1))))) ==> !abort_flag;
+ensures old(b#Boolean(Boolean(i#Integer(arg0) < i#Integer(arg1)))) ==> abort_flag;
+{
+    // declare local variables
+    var t0: Value; // IntegerType()
+    var t1: Value; // IntegerType()
+    var t2: Value; // IntegerType()
+    var t3: Value; // IntegerType()
+    var t4: Value; // BooleanType()
+    var t5: Value; // BooleanType()
+    var t6: Value; // IntegerType()
+
+    var tmp: Value;
+    var old_size: int;
+
+    var saved_m: Memory;
+    assume !abort_flag;
+    saved_m := m;
+
+    // assume arguments are of correct types
+    assume is#Integer(arg0);
+    assume is#Integer(arg1);
+
+    old_size := local_counter;
+    local_counter := local_counter + 7;
+    m := UpdateLocal(m, old_size + 0, arg0);
+    m := UpdateLocal(m, old_size + 1, arg1);
+
+    // bytecode translation starts here
+    call tmp := CopyOrMoveValue(GetLocal(m, old_size + 0));
+    m := UpdateLocal(m, old_size + 2, tmp);
+
+    call tmp := CopyOrMoveValue(GetLocal(m, old_size + 1));
+    m := UpdateLocal(m, old_size + 3, tmp);
+
+    call tmp := Gt(GetLocal(m, old_size + 2), GetLocal(m, old_size + 3));
+    m := UpdateLocal(m, old_size + 4, tmp);
+
+    call tmp := Not(GetLocal(m, old_size + 4));
+    m := UpdateLocal(m, old_size + 5, tmp);
+
+    tmp := GetLocal(m, old_size + 5);
+    if (!b#Boolean(tmp)) { goto Label_7; }
+
+    call tmp := LdConst(1);
+    m := UpdateLocal(m, old_size + 6, tmp);
+
+    goto Label_Abort;
+
+Label_7:
+    return;
+
+Label_Abort:
+    abort_flag := true;
+    m := saved_m;
+}
+
+procedure TestAbortIf_abort6_verify (arg0: Value, arg1: Value) returns ()
+{
+    call TestAbortIf_abort6(arg0, arg1);
+}
+
+procedure {:inline 1} TestAbortIf_abort7 (arg0: Value, arg1: Value) returns ()
+requires ExistsTxnSenderAccount(m, txn);
+ensures old(!(b#Boolean(Boolean(i#Integer(arg0) < i#Integer(arg1)))) && (b#Boolean(Boolean(i#Integer(arg0) >= i#Integer(arg1))))) ==> !abort_flag;
+ensures old(b#Boolean(Boolean(i#Integer(arg0) < i#Integer(arg1)))) ==> abort_flag;
+{
+    // declare local variables
+    var t0: Value; // IntegerType()
+    var t1: Value; // IntegerType()
+    var t2: Value; // IntegerType()
+    var t3: Value; // IntegerType()
+    var t4: Value; // BooleanType()
+    var t5: Value; // BooleanType()
+    var t6: Value; // IntegerType()
+
+    var tmp: Value;
+    var old_size: int;
+
+    var saved_m: Memory;
+    assume !abort_flag;
+    saved_m := m;
+
+    // assume arguments are of correct types
+    assume is#Integer(arg0);
+    assume is#Integer(arg1);
+
+    old_size := local_counter;
+    local_counter := local_counter + 7;
+    m := UpdateLocal(m, old_size + 0, arg0);
+    m := UpdateLocal(m, old_size + 1, arg1);
+
+    // bytecode translation starts here
+    call tmp := CopyOrMoveValue(GetLocal(m, old_size + 0));
+    m := UpdateLocal(m, old_size + 2, tmp);
+
+    call tmp := CopyOrMoveValue(GetLocal(m, old_size + 1));
+    m := UpdateLocal(m, old_size + 3, tmp);
+
+    call tmp := Gt(GetLocal(m, old_size + 2), GetLocal(m, old_size + 3));
+    m := UpdateLocal(m, old_size + 4, tmp);
+
+    call tmp := Not(GetLocal(m, old_size + 4));
+    m := UpdateLocal(m, old_size + 5, tmp);
+
+    tmp := GetLocal(m, old_size + 5);
+    if (!b#Boolean(tmp)) { goto Label_7; }
+
+    call tmp := LdConst(1);
+    m := UpdateLocal(m, old_size + 6, tmp);
+
+    goto Label_Abort;
+
+Label_7:
+    return;
+
+Label_Abort:
+    abort_flag := true;
+    m := saved_m;
+}
+
+procedure TestAbortIf_abort7_verify (arg0: Value, arg1: Value) returns ()
+{
+    call TestAbortIf_abort7(arg0, arg1);
+}
+
+procedure {:inline 1} TestAbortIf_abort8 (arg0: Value, arg1: Value) returns (ret0: Value)
+requires ExistsTxnSenderAccount(m, txn);
+ensures !abort_flag ==> b#Boolean(Boolean((ret0) == (Boolean(true))));
+ensures old(!(b#Boolean(Boolean(i#Integer(arg0) < i#Integer(arg1)))) && (b#Boolean(Boolean(i#Integer(arg0) > i#Integer(arg1))))) ==> !abort_flag;
+ensures old(b#Boolean(Boolean(i#Integer(arg0) < i#Integer(arg1)))) ==> abort_flag;
+{
+    // declare local variables
+    var t0: Value; // IntegerType()
+    var t1: Value; // IntegerType()
+    var t2: Value; // IntegerType()
+    var t3: Value; // IntegerType()
+    var t4: Value; // BooleanType()
+    var t5: Value; // BooleanType()
+    var t6: Value; // IntegerType()
+    var t7: Value; // IntegerType()
+    var t8: Value; // IntegerType()
+    var t9: Value; // IntegerType()
+    var t10: Value; // BooleanType()
+
+    var tmp: Value;
+    var old_size: int;
+
+    var saved_m: Memory;
+    assume !abort_flag;
+    saved_m := m;
+
+    // assume arguments are of correct types
+    assume is#Integer(arg0);
+    assume is#Integer(arg1);
+
+    old_size := local_counter;
+    local_counter := local_counter + 11;
+    m := UpdateLocal(m, old_size + 0, arg0);
+    m := UpdateLocal(m, old_size + 1, arg1);
+
+    // bytecode translation starts here
+    call tmp := CopyOrMoveValue(GetLocal(m, old_size + 0));
+    m := UpdateLocal(m, old_size + 2, tmp);
+
+    call tmp := CopyOrMoveValue(GetLocal(m, old_size + 1));
+    m := UpdateLocal(m, old_size + 3, tmp);
+
+    call tmp := Gt(GetLocal(m, old_size + 2), GetLocal(m, old_size + 3));
+    m := UpdateLocal(m, old_size + 4, tmp);
+
+    call tmp := Not(GetLocal(m, old_size + 4));
+    m := UpdateLocal(m, old_size + 5, tmp);
+
+    tmp := GetLocal(m, old_size + 5);
+    if (!b#Boolean(tmp)) { goto Label_7; }
+
+    call tmp := LdConst(1);
+    m := UpdateLocal(m, old_size + 6, tmp);
+
+    goto Label_Abort;
+
+Label_7:
+    call tmp := CopyOrMoveValue(GetLocal(m, old_size + 0));
+    m := UpdateLocal(m, old_size + 7, tmp);
+
+    call tmp := CopyOrMoveValue(GetLocal(m, old_size + 7));
+    m := UpdateLocal(m, old_size + 1, tmp);
+
+    call tmp := CopyOrMoveValue(GetLocal(m, old_size + 0));
+    m := UpdateLocal(m, old_size + 8, tmp);
+
+    call tmp := CopyOrMoveValue(GetLocal(m, old_size + 1));
+    m := UpdateLocal(m, old_size + 9, tmp);
+
+    tmp := Boolean(IsEqual(GetLocal(m, old_size + 8), GetLocal(m, old_size + 9)));
+    m := UpdateLocal(m, old_size + 10, tmp);
+
+    ret0 := GetLocal(m, old_size + 10);
+    return;
+
+Label_Abort:
+    abort_flag := true;
+    m := saved_m;
+    ret0 := DefaultValue;
+}
+
+procedure TestAbortIf_abort8_verify (arg0: Value, arg1: Value) returns (ret0: Value)
+{
+    call ret0 := TestAbortIf_abort8(arg0, arg1);
+}
+
+procedure {:inline 1} TestAbortIf_abort9 (arg0: Value, arg1: Value) returns ()
+requires ExistsTxnSenderAccount(m, txn);
+ensures !abort_flag ==> b#Boolean(Boolean((arg0) == (arg1)));
+ensures old(!(b#Boolean(Boolean(i#Integer(arg0) > i#Integer(arg1))) || b#Boolean(Boolean(i#Integer(arg0) < i#Integer(arg1))))) ==> !abort_flag;
+ensures old(b#Boolean(Boolean(i#Integer(arg0) > i#Integer(arg1))) || b#Boolean(Boolean(i#Integer(arg0) < i#Integer(arg1)))) ==> abort_flag;
+{
+    // declare local variables
+    var t0: Value; // IntegerType()
+    var t1: Value; // IntegerType()
+    var t2: Value; // IntegerType()
+    var t3: Value; // IntegerType()
+    var t4: Value; // BooleanType()
+    var t5: Value; // BooleanType()
+    var t6: Value; // IntegerType()
+
+    var tmp: Value;
+    var old_size: int;
+
+    var saved_m: Memory;
+    assume !abort_flag;
+    saved_m := m;
+
+    // assume arguments are of correct types
+    assume is#Integer(arg0);
+    assume is#Integer(arg1);
+
+    old_size := local_counter;
+    local_counter := local_counter + 7;
+    m := UpdateLocal(m, old_size + 0, arg0);
+    m := UpdateLocal(m, old_size + 1, arg1);
+
+    // bytecode translation starts here
+    call tmp := CopyOrMoveValue(GetLocal(m, old_size + 0));
+    m := UpdateLocal(m, old_size + 2, tmp);
+
+    call tmp := CopyOrMoveValue(GetLocal(m, old_size + 1));
+    m := UpdateLocal(m, old_size + 3, tmp);
+
+    call tmp := Gt(GetLocal(m, old_size + 2), GetLocal(m, old_size + 3));
+    m := UpdateLocal(m, old_size + 4, tmp);
+
+    call tmp := Not(GetLocal(m, old_size + 4));
+    m := UpdateLocal(m, old_size + 5, tmp);
+
+    tmp := GetLocal(m, old_size + 5);
+    if (!b#Boolean(tmp)) { goto Label_7; }
+
+    call tmp := LdConst(1);
+    m := UpdateLocal(m, old_size + 6, tmp);
+
+    goto Label_Abort;
+
+Label_7:
+    return;
+
+Label_Abort:
+    abort_flag := true;
+    m := saved_m;
+}
+
+procedure TestAbortIf_abort9_verify (arg0: Value, arg1: Value) returns ()
+{
+    call TestAbortIf_abort9(arg0, arg1);
+}
